Weidenbach_Book/IsaSAT/IsaSAT_Restart_Reduce.thy
@@ -3206,19 +3206,14 @@ definition isasat_GC_clauses_pre_wl_D :: \<open>isasat \<Rightarrow> bool\<close
   \<exists>T. (S, T) \<in> twl_st_heur_restart \<and> cdcl_GC_clauses_pre_wl T
   )\<close>
 
-definition reset_added_heur_st :: \<open>bool \<Rightarrow> isasat \<Rightarrow> isasat\<close> where
-  \<open>reset_added_heur_st b S =
-  (if b \<and> should_inprocess_st S then let heur = get_heur S in set_heur_wl_heur (schedule_next_inprocessing (reset_added_heur heur)) S else S)\<close>
+definition schedule_next_inprocessing_st :: \<open>bool \<Rightarrow> isasat \<Rightarrow> isasat\<close> where
+  \<open>schedule_next_inprocessing_st b S =
+  (if b \<and> should_inprocess_st S then let heur = get_heur S in set_heur_wl_heur (schedule_next_inprocessing (heur)) S else S)\<close>
 
-lemma [intro!]: \<open>heuristic_rel A heur \<Longrightarrow> heuristic_rel A (reset_added_heur heur)\<close>
-  by (auto simp: heuristic_rel_def heuristic_rel_stats_def
-    reset_added_heur_stats_def phase_saving_def
-    reset_added_heur_def)
-
-lemma reset_added_heur_st:
+lemma schedule_next_inprocessing_st:
   \<open>(S, T) \<in> twl_st_heur_restart''''u r u \<Longrightarrow>
-  (reset_added_heur_st b S, T) \<in> twl_st_heur_restart''''u r u\<close>
-  by (auto simp: reset_added_heur_st_def twl_st_heur_restart_def)
+  (schedule_next_inprocessing_st b S, T) \<in> twl_st_heur_restart''''u r u\<close>
+  by (auto simp: schedule_next_inprocessing_st_def twl_st_heur_restart_def)
 
 definition isasat_GC_clauses_wl_D :: \<open>bool \<Rightarrow> isasat \<Rightarrow> isasat nres\<close> where
 \<open>isasat_GC_clauses_wl_D = (\<lambda>inprocessing S. do {
@@ -3229,7 +3224,7 @@ definition isasat_GC_clauses_wl_D :: \<open>bool \<Rightarrow> isasat \<Rightarr
     ASSERT(length (get_clauses_wl_heur T) \<le> length (get_clauses_wl_heur S));
     ASSERT(\<forall>i \<in> set (get_tvdom T). i < length (get_clauses_wl_heur S));
     U \<leftarrow> rewatch_heur_and_reorder_st (empty_US_heur T);
-    RETURN (reset_added_heur_st inprocessing U)
+    RETURN (schedule_next_inprocessing_st inprocessing U)
   }
   else RETURN S})\<close>
 
@@ -3770,7 +3765,7 @@ lemma isasat_GC_clauses_wl_D:
   unfolding prod_rel_fst_snd_iff
     isasat_GC_clauses_wl_D_def cdcl_GC_clauses_wl_D_alt_def uncurry_def
   apply (refine_vcg isasat_GC_clauses_prog_wl_cdcl_remap_st[where r=r]
-    rewatch_heur_st_correct_watching reset_added_heur_st)
+    rewatch_heur_st_correct_watching schedule_next_inprocessing_st)
   subgoal unfolding isasat_GC_clauses_pre_wl_D_def by blast
   subgoal by fast
   apply assumption
